Disjointness of sets.

algebra/sts.v
@@ -26,17 +26,16 @@ Context {sts : stsT}.
 (** ** Step relations *)
 Inductive step : relation (state sts * tokens sts) :=
   | Step s1 s2 T1 T2 :
-     (* TODO: This asks for ⊥ on sets: T1 ⊥ T2 := T1 ∩ T2 ⊆ ∅. *)
-     prim_step s1 s2 → tok s1 ∩ T1 ≡ ∅ → tok s2 ∩ T2 ≡ ∅ →
+     prim_step s1 s2 → tok s1 ⊥ T1 → tok s2 ⊥ T2 →
      tok s1 ∪ T1 ≡ tok s2 ∪ T2 → step (s1,T1) (s2,T2).
 Notation steps := (rtc step).
 Inductive frame_step (T : tokens sts) (s1 s2 : state sts) : Prop :=
   | Frame_step T1 T2 :
-     T1 ∩ (tok s1 ∪ T) ≡ ∅ → step (s1,T1) (s2,T2) → frame_step T s1 s2.
+     T1 ⊥ tok s1 ∪ T → step (s1,T1) (s2,T2) → frame_step T s1 s2.
 
 (** ** Closure under frame steps *)
 Record closed (S : states sts) (T : tokens sts) : Prop := Closed {
-  closed_disjoint s : s ∈ S → tok s ∩ T ≡ ∅;
+  closed_disjoint s : s ∈ S → tok s ⊥ T;
   closed_step s1 s2 : s1 ∈ S → frame_step T s1 s2 → s2 ∈ S
 }.
 Definition up (s : state sts) (T : tokens sts) : states sts :=
@@ -50,6 +49,7 @@ Hint Extern 50 (equiv (A:=set _) _ _) => set_solver : sts.
 Hint Extern 50 (¬equiv (A:=set _) _ _) => set_solver : sts.
 Hint Extern 50 (_ ∈ _) => set_solver : sts.
 Hint Extern 50 (_ ⊆ _) => set_solver : sts.
+Hint Extern 50 (_ ⊥ _) => set_solver : sts.
 
 (** ** Setoids *)
 Instance framestep_mono : Proper (flip (⊆) ==> (=) ==> (=) ==> impl) frame_step.
@@ -60,10 +60,7 @@ Qed.
 Global Instance framestep_proper : Proper ((≡) ==> (=) ==> (=) ==> iff) frame_step.
 Proof. by intros ?? [??] ??????; split; apply framestep_mono. Qed.
 Instance closed_proper' : Proper ((≡) ==> (≡) ==> impl) closed.
-Proof.
-  intros ?? HT ?? HS; destruct 1;
-    constructor; intros until 0; rewrite -?HS -?HT; eauto.
-Qed.
+Proof. destruct 3; constructor; intros until 0; setoid_subst; eauto. Qed.
 Global Instance closed_proper : Proper ((≡) ==> (≡) ==> iff) closed.
 Proof. by split; apply closed_proper'. Qed.
 Global Instance up_preserving : Proper ((=) ==> flip (⊆) ==> (⊆)) up.
@@ -95,16 +92,16 @@ Proof.
   - apply Hstep2 with s3, Frame_step with T3 T4; auto with sts.
 Qed.
 Lemma step_closed s1 s2 T1 T2 S Tf :
-  step (s1,T1) (s2,T2) → closed S Tf → s1 ∈ S → T1 ∩ Tf ≡ ∅ →
-  s2 ∈ S ∧ T2 ∩ Tf ≡ ∅ ∧ tok s2 ∩ T2 ≡ ∅.
+  step (s1,T1) (s2,T2) → closed S Tf → s1 ∈ S → T1 ⊥ Tf →
+  s2 ∈ S ∧ T2 ⊥ Tf ∧ tok s2 ⊥ T2.
 Proof.
   inversion_clear 1 as [???? HR Hs1 Hs2]; intros [? Hstep]??; split_and?; auto.
   - eapply Hstep with s1, Frame_step with T1 T2; auto with sts.
   - set_solver -Hstep Hs1 Hs2.
 Qed.
 Lemma steps_closed s1 s2 T1 T2 S Tf :
-  steps (s1,T1) (s2,T2) → closed S Tf → s1 ∈ S → T1 ∩ Tf ≡ ∅ →
-  tok s1 ∩ T1 ≡ ∅ → s2 ∈ S ∧ T2 ∩ Tf ≡ ∅ ∧ tok s2 ∩ T2 ≡ ∅.
+  steps (s1,T1) (s2,T2) → closed S Tf → s1 ∈ S → T1 ⊥ Tf →
+  tok s1 ⊥ T1 → s2 ∈ S ∧ T2 ⊥ Tf ∧ tok s2 ⊥ T2.
 Proof.
   remember (s1,T1) as sT1 eqn:HsT1; remember (s2,T2) as sT2 eqn:HsT2.
   intros Hsteps; revert s1 T1 HsT1 s2 T2 HsT2.
@@ -120,8 +117,7 @@ Lemma subseteq_up_set S T : S ⊆ up_set S T.
 Proof. intros s ?; apply elem_of_bind; eauto using elem_of_up. Qed.
 Lemma up_up_set s T : up s T ≡ up_set {[ s ]} T.
 Proof. by rewrite /up_set collection_bind_singleton. Qed.
-Lemma closed_up_set S T :
-  (∀ s, s ∈ S → tok s ∩ T ≡ ∅) → closed (up_set S T) T.
+Lemma closed_up_set S T : (∀ s, s ∈ S → tok s ⊥ T) → closed (up_set S T) T.
 Proof.
   intros HS; unfold up_set; split.
   - intros s; rewrite !elem_of_bind; intros (s'&Hstep&Hs').
@@ -131,7 +127,7 @@ Proof.
   - intros s1 s2; rewrite /up; set_unfold; intros (s&?&?) ?; exists s.
     split; [eapply rtc_r|]; eauto.
 Qed.
-Lemma closed_up s T : tok s ∩ T ≡ ∅ → closed (up s T) T.
+Lemma closed_up s T : tok s ⊥ T → closed (up s T) T.
 Proof.
   intros; rewrite -(collection_bind_singleton (λ s, up s T) s).
   apply closed_up_set; set_solver.
@@ -188,7 +184,7 @@ Inductive sts_equiv : Equiv (car sts) :=
 Global Existing Instance sts_equiv.
 Global Instance sts_valid : Valid (car sts) := λ x,
   match x with
-  | auth s T => tok s ∩ T ≡ ∅
+  | auth s T => tok s ⊥ T
   | frag S' T => closed S' T ∧ S' ≢ ∅
   end.
 Global Instance sts_core : Core (car sts) := λ x,
@@ -198,11 +194,9 @@ Global Instance sts_core : Core (car sts) := λ x,
   end.
 Inductive sts_disjoint : Disjoint (car sts) :=
   | frag_frag_disjoint S1 S2 T1 T2 :
-     S1 ∩ S2 ≢ ∅ → T1 ∩ T2 ≡ ∅ → frag S1 T1 ⊥ frag S2 T2
-  | auth_frag_disjoint s S T1 T2 :
-     s ∈ S → T1 ∩ T2 ≡ ∅ → auth s T1 ⊥ frag S T2
-  | frag_auth_disjoint s S T1 T2 :
-     s ∈ S → T1 ∩ T2 ≡ ∅ → frag S T1 ⊥ auth s T2.
+     S1 ∩ S2 ≢ ∅ → T1 ⊥ T2 → frag S1 T1 ⊥ frag S2 T2
+  | auth_frag_disjoint s S T1 T2 : s ∈ S → T1 ⊥ T2 → auth s T1 ⊥ frag S T2
+  | frag_auth_disjoint s S T1 T2 : s ∈ S → T1 ⊥ T2 → frag S T1 ⊥ auth s T2.
 Global Existing Instance sts_disjoint.
 Global Instance sts_op : Op (car sts) := λ x1 x2,
   match x1, x2 with
@@ -216,6 +210,8 @@ Hint Extern 50 (equiv (A:=set _) _ _) => set_solver : sts.
 Hint Extern 50 (¬equiv (A:=set _) _ _) => set_solver : sts.
 Hint Extern 50 (_ ∈ _) => set_solver : sts.
 Hint Extern 50 (_ ⊆ _) => set_solver : sts.
+Hint Extern 50 (_ ⊥ _) => set_solver : sts.
+
 Global Instance sts_equivalence: Equivalence ((≡) : relation (car sts)).
 Proof.
   split.
@@ -303,11 +299,11 @@ Global Instance sts_frag_up_proper s : Proper ((≡) ==> (≡)) (sts_frag_up s).
 Proof. intros T1 T2 HT. by rewrite /sts_frag_up HT. Qed.
 
 (** Validity *)
-Lemma sts_auth_valid s T : ✓ sts_auth s T ↔ tok s ∩ T ≡ ∅.
+Lemma sts_auth_valid s T : ✓ sts_auth s T ↔ tok s ⊥ T.
 Proof. done. Qed.
 Lemma sts_frag_valid S T : ✓ sts_frag S T ↔ closed S T ∧ S ≢ ∅.
 Proof. done. Qed.
-Lemma sts_frag_up_valid s T : tok s ∩ T ≡ ∅ → ✓ sts_frag_up s T.
+Lemma sts_frag_up_valid s T : tok s ⊥ T → ✓ sts_frag_up s T.
 Proof. intros. by apply sts_frag_valid; auto using closed_up, up_non_empty. Qed.
 
 Lemma sts_auth_frag_valid_inv s S T1 T2 :
@@ -335,7 +331,7 @@ Proof.
 Qed.
 
 Lemma sts_op_frag S1 S2 T1 T2 :
-  T1 ∩ T2 ≡ ∅ → sts.closed S1 T1 → sts.closed S2 T2 →
+  T1 ⊥ T2 → sts.closed S1 T1 → sts.closed S2 T2 →
   sts_frag (S1 ∩ S2) (T1 ∪ T2) ≡ sts_frag S1 T1 ⋅ sts_frag S2 T2.
 Proof.
   intros HT HS1 HS2. rewrite /sts_frag.
@@ -390,7 +386,7 @@ Qed.
 Lemma sts_frag_included S1 S2 T1 T2 :
   closed S2 T2 → S2 ≢ ∅ →
   (sts_frag S1 T1 ≼ sts_frag S2 T2) ↔
-  (closed S1 T1 ∧ S1 ≢ ∅ ∧ ∃ Tf, T2 ≡ T1 ∪ Tf ∧ T1 ∩ Tf ≡ ∅ ∧
+  (closed S1 T1 ∧ S1 ≢ ∅ ∧ ∃ Tf, T2 ≡ T1 ∪ Tf ∧ T1 ⊥ Tf ∧
                                  S2 ≡ S1 ∩ up_set S2 Tf).
 Proof.
   intros ??; split.
