prelude/fin_map_dom.v
@@ -74,15 +74,14 @@ Proof. rewrite not_elem_of_dom. apply delete_partial_alter. Qed.
 Lemma delete_insert_dom {A} (m : M A) i x :
   i ∉ dom D m → delete i (<[i:=x]>m) = m.
 Proof. rewrite not_elem_of_dom. apply delete_insert. Qed.
-Lemma map_disjoint_dom {A} (m1 m2 : M A) : m1 ⊥ₘ m2 ↔ dom D m1 ∩ dom D m2 ≡ ∅.
+Lemma map_disjoint_dom {A} (m1 m2 : M A) : m1 ⊥ₘ m2 ↔ dom D m1 ⊥ dom D m2.
 Proof.
-  rewrite map_disjoint_spec, elem_of_equiv_empty.
-  setoid_rewrite elem_of_intersection.
+  rewrite map_disjoint_spec, elem_of_disjoint.
   setoid_rewrite elem_of_dom. unfold is_Some. naive_solver.
 Qed.
-Lemma map_disjoint_dom_1 {A} (m1 m2 : M A) : m1 ⊥ₘ m2 → dom D m1 ∩ dom D m2 ≡ ∅.
+Lemma map_disjoint_dom_1 {A} (m1 m2 : M A) : m1 ⊥ₘ m2 → dom D m1 ⊥ dom D m2.
 Proof. apply map_disjoint_dom. Qed.
-Lemma map_disjoint_dom_2 {A} (m1 m2 : M A) : dom D m1 ∩ dom D m2 ≡ ∅ → m1 ⊥ₘ m2.
+Lemma map_disjoint_dom_2 {A} (m1 m2 : M A) : dom D m1 ⊥ dom D m2 → m1 ⊥ₘ m2.
 Proof. apply map_disjoint_dom. Qed.
 Lemma dom_union {A} (m1 m2 : M A) : dom D (m1 ∪ m2) ≡ dom D m1 ∪ dom D m2.
 Proof.
@@ -90,8 +89,7 @@ Proof.
   unfold is_Some. setoid_rewrite lookup_union_Some_raw.
   destruct (m1 !! i); naive_solver.
 Qed.
-Lemma dom_intersection {A} (m1 m2 : M A) :
-  dom D (m1 ∩ m2) ≡ dom D m1 ∩ dom D m2.
+Lemma dom_intersection {A} (m1 m2: M A) : dom D (m1 ∩ m2) ≡ dom D m1 ∩ dom D m2.
 Proof.
   apply elem_of_equiv. intros i. rewrite elem_of_intersection, !elem_of_dom.
   unfold is_Some. setoid_rewrite lookup_intersection_Some. naive_solver.
